src/simulations/SimulationUtils.v
@@ -30,7 +30,7 @@ Proof. intros ?. apply rt_trans. Qed.
 
 Inductive measured_closure {A : Type} (R : nat -> A -> A -> Prop) : nat -> A -> A -> Prop :=
   | MC_base n x y : R n x y -> measured_closure R n x y
-  | MC_refl n x : measured_closure R n x x
+  | MC_refl x : measured_closure R 0 x x
   | MC_trans m n x y z :
       measured_closure R m x y -> measured_closure R n y z -> measured_closure R (m + n) x z
 .
@@ -38,17 +38,6 @@ Inductive measured_closure {A : Type} (R : nat -> A -> A -> Prop) : nat -> A -> 
 (* Now let's assume that a relation <_n is equipped with an integer measure.
  * We can define a reflexive-transitive closure that takes the measure into account. *)
 Notation "R ^{ n }" := (measured_closure R n).
-
-Global Instance measured_closure_refl A R n : Reflexive (@measured_closure A R n).
-Proof. intros ?. apply MC_refl. Qed.
-
-Lemma measured_closure_over_approx {A} R m n x y :
-  m <= n -> R^{m} x y -> (@measured_closure A R n x y).
-Proof.
-  intros ? ?. replace n with (m + (n - m)); [ | lia]. eapply MC_trans.
-  - eassumption.
-  - reflexivity.
-Qed.
 
 Definition equiv_rel {A B} (R0 R1 : A -> B -> Prop) := forall a b, R0 a b <-> R1 a b.
 
@@ -61,7 +50,7 @@ Proof.
   intros x y. split.
   - induction 1 as [x y | | x y z ? IH0 ? IH1].
     + destruct (H x y) as ((n & ?) & _); [assumption | ]. exists n. constructor. assumption.
-    + exists 0. reflexivity.
+    + exists 0. apply MC_refl.
     + destruct IH0 as (m & ?). destruct IH1 as (n & ?). exists (m + n).
       eapply MC_trans; eassumption.
   - intros (n & G). induction G.
@@ -71,16 +60,30 @@ Proof.
 Qed.
 
 (* TODO: name *)
-Lemma measure_closure_cases {A} (R : nat -> A -> A -> Prop) n x z :
-  R^{n} x z -> x = z \/ exists p q y, R^{p} x y /\ R q y z /\ p + q <= n.
+Lemma measure_closure_cases_left {A} (R : nat -> A -> A -> Prop) n x z :
+  R^{n} x z -> x = z /\ n = 0 \/ exists p q y, R^{p} x y /\ R q y z /\ n = p + q.
 Proof.
   induction 1 as [n x z | | m n x y z ? IH0 ? IH1].
   - right. exists 0, n, x. auto using MC_refl.
   - auto.
-  - destruct IH1 as [-> | (p & q & y' & ? & ? & ?)].
-    + destruct IH0 as [ | (p & q & y & ? & ? & ?)]; [auto | ].
+  - destruct IH1 as [(-> & ->) | (p & q & y' & ? & ? & ->)].
+    + destruct IH0 as [(-> & ->) | (p & q & y & ? & ? & ->)]; [auto | ].
       right. exists p, q, y. repeat split; try assumption. lia.
-    + right. eexists _, _, y'. repeat split; [ | eassumption | ].
+    + right. eexists _, q, y'. repeat split; [ | eassumption | ].
+      * eapply MC_trans; eassumption.
+      * lia.
+Qed.
+
+Lemma measure_closure_cases_right {A} (R : nat -> A -> A -> Prop) n x z :
+  R^{n} x z -> x = z /\ n = 0 \/ exists p q y, R p x y /\ R^{q} y z /\ n = p + q.
+Proof.
+  induction 1 as [n x z | | m n x y z ? IH0 ? IH1].
+  - right. exists n, 0, z. auto using MC_refl.
+  - auto.
+  - destruct IH0 as [(<- & ->) | (p & q & y' & ? & ? & ->)].
+    + destruct IH1 as [(<- & ->) | (p & q & y & ? & ? & ->)]; [auto | ].
+      right. exists p, q, y. auto.
+    + right. eexists p, _, y'. repeat split; [eassumption | | ].
       * eapply MC_trans; eassumption.
       * lia.
 Qed.
@@ -218,188 +221,13 @@ Section LeqValStateUtils.
   Qed.
 End LeqValStateUtils.
 
+(** Tactics to prove commutation of reorganizations. *)
+(* TODO: document it *)
 Lemma leq_step_right {S} {R : relation S} Sl Sm Sr : R Sm Sr -> R^* Sl Sm -> R^* Sl Sr.
 Proof. intros. transitivity Sm; [ | constructor]; assumption. Qed.
 
 Lemma leq_step_left {S} {R : relation S} Sl Sm Sr : R Sl Sm -> R^* Sm Sr -> R^* Sl Sr.
 Proof. intros. transitivity Sm; [constructor | ]; assumption. Qed.
-
-(** Tactics to prove commutation of reorganizations. *)
-(* TODO: document it *)
-Lemma prove_reorg_step {S} {reorg leq : relation S} S0 S1 Sr:
-  reorg S0 S1 -> (exists Sl, leq Sl Sr /\ reorg^* S1 Sl) ->
-  exists Sl, leq Sl Sr /\ reorg^* S0 Sl.
-Proof.
-  intros ? (Sl & ? & ?). exists Sl. split; [assumption | ].
-  etransitivity; [constructor | ]; eassumption.
-Qed.
-
-Lemma prove_reorg_steps {S} {reorg leq : relation S} S0 S1 Sr:
-  reorg^* S0 S1 -> (exists Sl, leq Sl Sr /\ reorg^* S1 Sl) ->
-  exists Sl, leq Sl Sr /\ reorg^* S0 Sl.
-Proof.
-  intros ? (Sl & ? & ?). exists Sl. split; [assumption | ].
-  etransitivity; eassumption.
-Qed.
-
-Ltac reorg_step := eapply prove_reorg_step.
-Ltac reorg_steps := eapply prove_reorg_steps.
-Ltac reorg_done := eexists; split; [ | reflexivity].
-
-Section Leq.
-  Context {state : Type}.
-  Context {equiv : state -> state -> Prop}.
-  Context `{Reflexive _ equiv}.
-  Context `{Transitive _ equiv}.
-  Context (leq_base : state -> state -> Prop).
-  Context (sim_leq_base_equiv : forward_simulation leq_base leq_base equiv equiv).
-
-  Definition leq := chain equiv leq_base^*.
-
-  Global Instance reflexive_leq : Reflexive leq.
-  Proof. intros x. exists x. split; reflexivity. Qed.
-
-  Lemma sim_leq_equiv : forward_simulation leq_base^* leq_base^* equiv equiv.
-  Proof.
-    intros a b red_ab a' Leq_a_a'. revert b red_ab.
-    induction Leq_a_a' as [? ? Leq_a_a' | | a2 a1 a0 _ IH0 _ IH1].
-    - intros. specialize (sim_leq_base_equiv _ _ red_ab _ Leq_a_a').
-      destruct sim_leq_base_equiv as (d & ? & ?). exists d. split; [constructor | ]; assumption.
-    - intros. eexists. split; [reflexivity | eassumption].
-    - intros b0 Red_a0_b0.
-      destruct (IH1 _ Red_a0_b0) as (b1 & ? & Red_a1_b1).
-      destruct (IH0 _ Red_a1_b1) as (b2 & ? & Red_a2_b2).
-      exists b2. split; [ | assumption]. transitivity b1; assumption.
-  Qed.
-
-  Global Instance transitive_leq : Transitive leq.
-  Proof.
-    intros x y z (y' & ? & leq_y'_y) (z' & equiv_y_z' & ?).
-    pose proof (sim_leq_equiv _ _ equiv_y_z' _ leq_y'_y) as G.
-    destruct G as (z'' & ? & ?). exists z''. split.
-    - transitivity y'; assumption.
-    - transitivity z'; assumption.
-  Qed.
-
-  Context (reorg : state -> state -> Prop).
-  Context (measure : state -> nat).
-  Context (leq_base_n : nat -> state -> state -> Prop).
-  Definition leq_n n := chain equiv (measured_closure leq_base_n n).
-
-  Hypothesis (leq_decreasing : forall n a b, leq_base_n n a b -> measure a < measure b + n).
-  Hypothesis (reorg_decreasing : forall a b, reorg a b -> measure b < measure a).
-
-  Lemma leq_clos_decreasing : forall S S', reorg^* S S' -> measure S' <= measure S.
-  Proof. intros ? ? Hreorg. induction Hreorg; eauto using Nat.lt_le_incl, Nat.le_trans. Qed.
-
-  Hypothesis (reorg_preserves_equiv : forward_simulation equiv equiv reorg reorg).
-  Lemma reorgs_preserve_equiv : forward_simulation equiv equiv reorg^* reorg^*.
-  Proof.
-  intros a b. induction 1 as [? ? Hreorg | | a0 a1 a2 _ IH0 _ IH1].
-  - intros ? Hequiv. specialize (reorg_preserves_equiv _ _ Hreorg _ Hequiv).
-    destruct reorg_preserves_equiv as (d & ? & ?). exists d.
-    split; [ | constructor]; assumption.
-  - intros. eexists. split; [ | reflexivity]. assumption.
-  - intros b0 equiv_b0_a0.
-    destruct (IH0 _ equiv_b0_a0) as (b1 & Red_b1_a1 & ?).
-    destruct (IH1 _ Red_b1_a1) as (b2 & Red_b2_a1 & ?).
-    exists b2. split; [assumption | ]. transitivity b1; assumption.
-  Qed.
-
-  Context (sim_equiv_leq_base_n :
-    forall n, forward_simulation (leq_base_n n) (leq_base_n n) equiv equiv).
-
-  Lemma leq_n_cases n Sl Sr (G : leq_n n Sl Sr) :
-    (equiv Sl Sr) \/
-    (exists p q Sm, leq_n p Sl Sm /\ leq_base_n q Sm Sr /\ p + q <= n).
-  Proof.
-    destruct G as (Sr' & Gequiv & Gcases%measure_closure_cases).
-    destruct Gcases as [-> | (p & q & Sm & ? & G & ?)].
-    - left. assumption.
-    - right. exists p, q, Sm. firstorder.
-  Qed.
-
-  Lemma sim_equiv_leq_n n : forward_simulation (leq_base_n^{n}) (leq_base_n^{n}) equiv equiv.
-  Proof.
-    intros a b equiv_ab a' Leq_a'_a. revert b equiv_ab.
-    induction Leq_a'_a as [n ? ? Leq_a'_a | | p q a2 a1 a0 _ IH0 _ IH1].
-    - intros. specialize (sim_equiv_leq_base_n n _ _ equiv_ab _ Leq_a'_a).
-      destruct sim_equiv_leq_base_n as (d & ? & ?). exists d. split; [constructor | ]; assumption.
-    - intros. eexists. split; [reflexivity | eassumption].
-    - intros b0 equiv_a0_b0.
-      destruct (IH1 _ equiv_a0_b0) as (b1 & ? & equiv_a1_b1).
-      destruct (IH0 _ equiv_a1_b1) as (b2 & ? & equiv_a2_b2).
-      exists b2. split; [ | assumption]. eapply MC_trans; eassumption.
-  Qed.
-
-  Lemma leq_n_trans Sl Sm Sr p q n :
-    leq_n p Sl Sm -> leq_n q Sm Sr -> p + q <= n -> leq_n n Sl Sr.
-  Proof.
-    intros (S'l & ? & leq_S'l_Sm) (S'm & equiv_Sm_S'm & ?).
-    pose proof (sim_equiv_leq_n p _ _ equiv_Sm_S'm _ leq_S'l_Sm) as (S''l & ? & ?).
-    intros ?. exists S''l. split.
-    - transitivity S'l; assumption.
-    - eapply measured_closure_over_approx; [ eassumption |].
-      eapply MC_trans; eassumption.
-  Qed.
-
-  Lemma measured_preservation_reorg_l
-    (G : forall n, forward_simulation (leq_base_n n) (leq_n n) reorg reorg^*) :
-    forall n, forward_simulation (leq_n n) (leq_n n) reorg^* reorg^*.
-  Proof.
-    intros n Sr. remember (measure Sr + n) as N eqn:EQN.
-    revert n Sr EQN. induction N as [? IH] using lt_wf_ind.
-    intros n Sr -> S''r reorg_Sr_S''r Sl leq_Sl_Sr.
-    destruct reorg_Sr_S''r as [ | Sr S'r S''r reorg_Sr_S'r ? _] using clos_refl_trans_ind_right'.
-    { eexists. split; [eassumption | reflexivity]. }
-    apply leq_n_cases in leq_Sl_Sr.
-    destruct leq_Sl_Sr as [Hequiv | (p & q & Sm & leq_Sl_Sm & leq_Sm_Sr & ?)].
-    { eapply reorgs_preserve_equiv in Hequiv.
-      - destruct Hequiv as (Sl' & ? & ?). exists Sl'. split; [ | assumption].
-        eexists. split; [eassumption | reflexivity].
-      - transitivity S'r; [constructor | ]; assumption. }
-    specialize (G q _ _ reorg_Sr_S'r _ leq_Sm_Sr).
-    destruct G as (S'm & leq_S'm_S'r & reorg_Sm_S'm).
-    specialize (leq_decreasing _ _ _ leq_Sm_Sr).
-    edestruct IH with (Sr := Sm) as (S'l & ? & ?);
-      [ | reflexivity | eassumption.. | ];
-      [lia | ].
-    pose proof (reorg_decreasing _ _ reorg_Sr_S'r).
-    edestruct IH with (Sr := S'r) as (S''m & ? & ?);
-      [ | reflexivity | eassumption.. | ];
-      [lia | ].
-    pose proof (leq_clos_decreasing _ _ reorg_Sm_S'm).
-    edestruct IH with (Sr := S'm) as (S''l & ? & ?);
-      [ | reflexivity | eassumption.. | ]. lia.
-    exists S''l. split.
-    - eapply leq_n_trans; eassumption.
-    - transitivity S'l; assumption.
-  Qed.
-
-  Context (leq_base_is_leq_base_n : forall Sl Sr, leq_base Sl Sr <-> exists n, leq_base_n n Sl Sr).
-
-  Lemma leq_n_is_leq Sl Sr : leq Sl Sr <-> exists n, leq_n n Sl Sr.
-  Proof.
-    split.
-    - intros (Sl' & Hequiv & Hleq).
-      rewrite measured_closure_equiv in Hleq by exact leq_base_is_leq_base_n.
-      destruct Hleq as (n & Hleq). exists n, Sl'. auto.
-    - intros (n & Sl' & Hequiv & Hleq). exists Sl'. split; [assumption | ].
-      rewrite measured_closure_equiv by exact leq_base_is_leq_base_n.
-      exists n. exact Hleq.
-  Qed.
-
-  Corollary preservation_reorg_l
-    (G : forall n, forward_simulation (leq_base_n n) (leq_n n) reorg reorg^*) :
-    forward_simulation leq leq reorg^* reorg^*.
-  Proof.
-    intros Sr S'l reorg_Sr_S'r Sl leq_Sl_Sr.
-    rewrite leq_n_is_leq in leq_Sl_Sr. destruct leq_Sl_Sr as (n & leq_n_Sl_Sr).
-    pose proof (measured_preservation_reorg_l G _ _ _ reorg_Sr_S'r _ leq_n_Sl_Sr)
-      as (Sl' & ? & ?).
-    exists Sl'. split; [ | assumption]. rewrite leq_n_is_leq. exists n. assumption.
-  Qed.
-End Leq.
 
 Section WellFormedSimulations.
   Context {state : Type}.
@@ -479,8 +307,180 @@ Section WellFormedSimulations.
   Qed.
 End WellFormedSimulations.
 
-Definition rel_compose {A B C : Type} (R : A -> B -> Prop) (S : B -> C -> Prop) a c :=
-  exists b, R a b /\ S b c.
+(** Simulation principles for LLBC\# and LLBC+, taking into account equivalence. *)
+Section SymbolicSimulations.
+  Context {state : Type}.
+  Context {equiv : state -> state -> Prop}.
+  Context `{Reflexive _ equiv}.
+  Context `{Transitive _ equiv}.
+  Context (leq_base : state -> state -> Prop).
+  Context (sim_leq_base_equiv : forward_simulation leq_base leq_base equiv equiv).
+
+  Definition leq := chain equiv leq_base^*.
+
+  Global Instance reflexive_leq : Reflexive leq.
+  Proof. intros x. exists x. split; reflexivity. Qed.
+
+  Lemma sim_leq_equiv : forward_simulation leq_base^* leq_base^* equiv equiv.
+  Proof.
+    intros a b red_ab a' Leq_a_a'. revert b red_ab.
+    induction Leq_a_a' as [? ? Leq_a_a' | | a2 a1 a0 _ IH0 _ IH1].
+    - intros. specialize (sim_leq_base_equiv _ _ red_ab _ Leq_a_a').
+      destruct sim_leq_base_equiv as (d & ? & ?). exists d. split; [constructor | ]; assumption.
+    - intros. eexists. split; [reflexivity | eassumption].
+    - intros b0 Red_a0_b0.
+      destruct (IH1 _ Red_a0_b0) as (b1 & ? & Red_a1_b1).
+      destruct (IH0 _ Red_a1_b1) as (b2 & ? & Red_a2_b2).
+      exists b2. split; [ | assumption]. transitivity b1; assumption.
+  Qed.
+
+  Global Instance transitive_leq : Transitive leq.
+  Proof.
+    intros x y z (y' & ? & leq_y'_y) (z' & equiv_y_z' & ?).
+    pose proof (sim_leq_equiv _ _ equiv_y_z' _ leq_y'_y) as G.
+    destruct G as (z'' & ? & ?). exists z''. split.
+    - transitivity y'; assumption.
+    - transitivity z'; assumption.
+  Qed.
+
+  Context (measure : state -> nat).
+  Context (reorg : state -> state -> Prop).
+  Context (reorg_n : nat -> state -> state -> Prop).
+  Context (leq_base_n : nat -> state -> state -> Prop).
+  Definition leq_n n := chain equiv (measured_closure leq_base_n n).
+
+  Hypothesis (leq_decreasing : forall n a b, leq_base_n n a b -> measure a < measure b + n).
+  Hypothesis (reorg_decreasing : forall n a b, reorg_n n a b -> measure b + n < measure a).
+  (*Hypothesis (equiv_measure : forall S S', equiv S S' -> measure S = measure S').*)
+
+  Lemma reorgs_decreasing n S S' : reorg_n^{n} S S' -> measure S' + n <= measure S.
+  Proof. induction 1; [ | lia..]. apply Nat.lt_le_incl, reorg_decreasing. assumption. Qed.
+
+  Hypothesis (reorg_preserves_equiv :
+    forall n, forward_simulation equiv equiv (reorg_n n) (reorg_n n)
+  ).
+
+  Lemma reorgs_preserve_equiv n :
+    forward_simulation equiv equiv (reorg_n^{n}) (reorg_n^{n}).
+  Proof.
+    intros a b. induction 1 as [? ? ? Hreorg | | p q a0 a1 a2 ? IH0 ? IH1].
+    - intros ? Hequiv. specialize (reorg_preserves_equiv _ _ _ Hreorg _ Hequiv).
+      destruct reorg_preserves_equiv as (d & ? & ?). exists d.
+      split; [ | constructor]; assumption.
+    - intros. eexists. split; [eassumption | apply MC_refl].
+    - intros b0 equiv_b0_a0.
+      destruct (IH0 _ equiv_b0_a0) as (b1 & Red_b1_a1 & ?).
+      destruct (IH1 _ Red_b1_a1) as (b2 & Red_b2_a1 & ?).
+      exists b2. split; [assumption | ]. eapply MC_trans; eassumption.
+  Qed.
+
+  Context (sim_equiv_leq_base_n :
+    forall n, forward_simulation (leq_base_n n) (leq_base_n n) equiv equiv).
+
+  Lemma leq_n_cases n Sl Sr (G : leq_n n Sl Sr) :
+    (equiv Sl Sr) \/
+    (exists p q Sm, leq_n p Sl Sm /\ leq_base_n q Sm Sr /\ n = p + q).
+  Proof.
+    destruct G as (Sr' & Gequiv & Gcases%measure_closure_cases_left).
+    destruct Gcases as [(-> & ->) | (p & q & Sm & ? & G & ->)].
+    - left. assumption.
+    - right. exists p, q, Sm. firstorder.
+  Qed.
+
+  Lemma sim_equiv_leq_n n : forward_simulation (leq_base_n^{n}) (leq_base_n^{n}) equiv equiv.
+  Proof.
+    intros a b equiv_ab a' Leq_a'_a. revert b equiv_ab.
+    induction Leq_a'_a as [n ? ? Leq_a'_a | | p q a2 a1 a0 _ IH0 _ IH1].
+    - intros. specialize (sim_equiv_leq_base_n n _ _ equiv_ab _ Leq_a'_a).
+      destruct sim_equiv_leq_base_n as (d & ? & ?). exists d. split; [constructor | ]; assumption.
+    - intros. eexists. split; [apply MC_refl | eassumption].
+    - intros b0 equiv_a0_b0.
+      destruct (IH1 _ equiv_a0_b0) as (b1 & ? & equiv_a1_b1).
+      destruct (IH0 _ equiv_a1_b1) as (b2 & ? & equiv_a2_b2).
+      exists b2. split; [ | assumption]. eapply MC_trans; eassumption.
+  Qed.
+
+  Lemma leq_n_trans Sl Sm Sr p q : leq_n p Sl Sm -> leq_n q Sm Sr -> leq_n (p + q) Sl Sr.
+  Proof.
+    intros (S'l & ? & leq_S'l_Sm) (S'm & equiv_Sm_S'm & ?).
+    pose proof (sim_equiv_leq_n p _ _ equiv_Sm_S'm _ leq_S'l_Sm) as (S''l & ? & ?).
+    exists S''l. split.
+    - transitivity S'l; assumption.
+    - eapply MC_trans; eassumption.
+  Qed.
+
+  Context (local_commutation :
+    forall p Sh q S'h, reorg_n q Sh S'h -> forall Sl, leq_base_n p Sl Sh ->
+    exists r s S'l, leq_n r S'l S'h /\ reorg_n^{s} Sl S'l /\ r + s <= p + q
+  ).
+
+  Lemma measured_preservation_reorg_l :
+    forall p Sh q S'h, reorg_n^{q} Sh S'h -> forall Sl, leq_n p Sl Sh ->
+    exists r s S'l, leq_n r S'l S'h /\ reorg_n^{s} Sl S'l /\ r + s <= p + q.
+  Proof.
+    intros p Sr. remember (measure Sr + p) as N eqn:EQN.
+    revert p Sr EQN. induction N as [? IH] using lt_wf_ind.
+    intros ? Sr -> q S''r reorg_Sr_S''r Sl leq_Sl_Sr.
+    destruct (measure_closure_cases_right _ _ _ _ reorg_Sr_S''r)
+      as [(-> & ->) | (? & ? & S'r & reorg_Sr_S'r & ? & ->)].
+    { eexists _, _, _. repeat split; [eassumption | apply MC_refl | lia]. }
+    apply leq_n_cases in leq_Sl_Sr.
+    destruct leq_Sl_Sr as [Hequiv | (? & ? & Sm & leq_Sl_Sm & leq_Sm_Sr & ->)].
+    { eapply reorgs_preserve_equiv in Hequiv; [ | exact reorg_Sr_S''r].
+      destruct Hequiv as (Sl' & ? & ?).
+      eexists 0, _, Sl'. repeat split; [ | eassumption | lia].
+      eexists. split; [eassumption | apply MC_refl]. }
+    specialize (local_commutation _ _ _ _ reorg_Sr_S'r _ leq_Sm_Sr).
+    destruct local_commutation as (? & ? & S'm & leq_S'm_S'r & reorg_Sm_S'm & ?).
+    pose proof (leq_decreasing _ _ _ leq_Sm_Sr).
+    edestruct IH with (Sr := Sm) as (? & ? & S'l & leq_S'l_S'm & reorg_Sl_S'l & ?);
+      [ | reflexivity | eassumption.. | ];
+      [lia | ].
+    pose proof (reorg_decreasing _ _ _ reorg_Sr_S'r).
+    edestruct IH with (Sr := S'r);
+      [ | reflexivity | eassumption | eapply leq_n_trans; eassumption | ];
+      [lia | ].
+    edestruct IH with (Sr := S'r) as (? & ? & S''m & ? & ? & ?);
+      [ | reflexivity | eassumption.. | ];
+      [lia | ].
+    pose proof (reorgs_decreasing _ _ _ reorg_Sm_S'm).
+    edestruct IH with (Sr := S'm) as (? & ? & S''l & ? & ? & ?);
+      [ | reflexivity | eassumption.. | ];
+      [lia | ].
+    eexists _, _, S''l. split; [ | split].
+    - eapply leq_n_trans; eassumption.
+    - eapply MC_trans; eassumption.
+    - lia.
+  Qed.
+
+  Context (leq_base_is_leq_base_n : forall Sl Sr, leq_base Sl Sr <-> exists n, leq_base_n n Sl Sr).
+  Context (reorg_is_reorg_n : forall Sl Sr, reorg Sl Sr <-> exists n, reorg_n n Sl Sr).
+
+  Lemma leq_n_is_leq Sl Sr : leq Sl Sr <-> exists n, leq_n n Sl Sr.
+  Proof.
+    split.
+    - intros (Sl' & Hequiv & Hleq).
+      rewrite measured_closure_equiv in Hleq by exact leq_base_is_leq_base_n.
+      destruct Hleq as (n & Hleq). exists n, Sl'. auto.
+    - intros (n & Sl' & Hequiv & Hleq). exists Sl'. split; [assumption | ].
+      rewrite measured_closure_equiv by exact leq_base_is_leq_base_n.
+      exists n. exact Hleq.
+  Qed.
+
+  Corollary preservation_reorg_l : forward_simulation leq leq reorg^* reorg^*.
+  Proof.
+    intros Sr S'l reorg_Sr_S'r Sl leq_Sl_Sr.
+    rewrite leq_n_is_leq in leq_Sl_Sr.
+    destruct leq_Sl_Sr as (p & leq_n_Sl_Sr).
+    rewrite measured_closure_equiv in reorg_Sr_S'r by exact reorg_is_reorg_n.
+    destruct reorg_Sr_S'r as (q & reorgs_n_Sr_S'r).
+    pose proof (measured_preservation_reorg_l _ _ _ _ reorgs_n_Sr_S'r _ leq_n_Sl_Sr)
+      as (r & s & Sl' & ? & ? & _).
+    exists Sl'. split.
+    - rewrite leq_n_is_leq. exists r. assumption.
+    - rewrite measured_closure_equiv by exact reorg_is_reorg_n. exists s. assumption.
+  Qed.
+End SymbolicSimulations.
 
 Lemma forward_simulation_closure A (E R : relation A) :
   forward_simulation E E R R -> forward_simulation E E R^* R^*.
