src/PathToSubtree.v
@@ -2516,11 +2516,12 @@ Hint Rewrite Nat2Z.inj_lt : weight.
 Hint Rewrite Nat2Z.inj_gt : weight.
 
 Hint Rewrite @sweight_sset using validity : weight.
+Hint Rewrite @vweight_vset using validity : weight.
 Hint Rewrite @sweight_add_anon using auto with weight : weight.
 
 (* When applying twice sweight_sset on a state of the form S.[p <- v].[q <- w], we end up
    with value S.[p <- v].[q], that we reduce using sset_sget_disj: *)
-Hint Rewrite @sset_sget_disj using eauto with spath : weight.
+Hint Rewrite @sset_sget_disj using solve_comp : weight.
 Hint Rewrite<- @sget_app : weight.
 
 Hint Rewrite @indicator_same : weight.
